add insertion algorithm (no splitting); prove list

src/Insert.v
@@ -5,12 +5,90 @@ From iris.prelude Require Import options.
 Require Import NaryTree.
 Require Import BPlusTree.
 
+Section nary_tree.
+
+  Fixpoint Insert_list (target : Z) (l : list Z) : list Z :=
+    match l with
+    | [] => [target]
+    | x :: xs => if Z.eqb x target
+               then x :: xs
+               else if Z.ltb x target
+                    then x :: Insert_list target xs
+                    else target :: x :: xs
+    end.
+
+  Fixpoint Insert_nary_tree (target : Z) (t : nary_tree) : nary_tree :=
+    match t with
+    | leaf interval vals => leaf interval (Insert_list target vals)
+    | node interval branches =>
+        node interval
+          ((fix insert_aux (l : list nary_tree) :=
+              match l with
+              | [] => [leaf (target, target) [target]]
+              | t :: ts =>
+                  let (low, high) := (match t with leaf interval _ | node interval _ => interval end) in
+                  if andb (Z.leb low target) (Z.leb target high)
+                  then Insert_nary_tree target t :: ts
+                  else t :: insert_aux ts
+              end) branches)
+    end.
+End nary_tree.
+
 Section bplus_tree.
   Section bplus_tree_algos.
 
+    Definition insert_list : val :=
+      rec: "insert_list" "arg" :=
+        let: "p" := Fst "arg" in
+        let: "target" := Snd "arg" in
+        match: "p" with
+          NONE =>
+            let: "ptr" := ref ("target", NONEV) in
+            SOME "ptr"
+        | SOME "l" =>
+            let: "val" := Fst !"l" in
+            if: "val" = "target"
+            then SOME "l"
+            else
+              if: (BinOp LtOp "val" "target")
+              then let: "new" := "insert_list" (Snd !"l", "target") in
+                   "l" <- ("val", "new");;
+                   SOME "l"
+              else SOME (ref ("target", SOME "l"))
+        end.
+
     Definition insert_bplus_tree : val :=
       rec: "insert_bplus_tree" "arg" :=
-        #().
+        let: "t" := Fst "arg" in
+        let: "target" := Snd "arg" in
+        match: "t" with
+          InjL "ptr" =>
+            let: "lhd" := Snd !"ptr" in
+            let: "new" := insert_list ("lhd", "target") in
+            (* should change interval here *)
+            "ptr" <- (Fst !"ptr", "new") ;;
+            "t"
+        | InjR "ptr" =>
+            let: "lhd" := Snd !"ptr" in
+            (rec: "insert_node_list" "arg" :=
+               let: "p" := Fst "arg" in
+               let: "target" := Snd "arg" in
+               match: "p" with
+                 NONE => #() (* create new leaf *)
+               | SOME "l" =>
+                   let: "val" := Fst !"l" in
+                   let: "interval" :=
+                     match: "val" with
+                       InjL "ptr" => Fst !"ptr"
+                     | InjR "ptr" => Fst !"ptr"
+                     end in
+                   let: "low" := Fst "interval" in
+                   let: "high" := Snd "interval" in
+                   if: (BinOp LeOp "low" "target") && (BinOp LeOp "target" "high")
+                   then "insert_bplus_tree" ("val", "target")
+                   else "insert_node_list" (Snd !"l", "target")
+               end) ("lhd", "target")
+        end%E.
   End bplus_tree_algos.
 
   Section bplus_tree_proofs.
@@ -32,9 +110,86 @@ Section bplus_tree.
       lia.
     Qed.
 
-    Theorem insert_bplus_tree_spec (t : tree_spec) (t_wf : tree_spec_wf b t) (v : val) (target : nat) :
-      {{{ is_bplus_tree b v t t_wf }}} insert_bplus_tree (v, #target)%V {{{ r, RET r; ⌜ r = #(In_bplus_tree target t) ⌝ ∗ is_bplus_tree b v t t_wf }}}.
+    Lemma insert_list_spec (v : val) (l : list tval) (target : tval):
+      {{{ is_list v (map (fun (x : tval) => #x) l) }}} insert_list (v, (#target))%V {{{ r, RET r; is_list r (map (fun (x : tval) => #x) (Insert_list target l)) }}}.
     Proof.
+      clear bpos.
+      iIntros (Φ) "Hl HPost".
+      iInduction l as [|x l] "IH" forall (Φ v); wp_rec; wp_pures.
+      - iDestruct "Hl" as "->".
+        wp_alloc ptr as "Hptr"; wp_pures.
+        iApply "HPost".
+        iExists ptr, (InjLV #()).
+        iFrame.
+        done.
+      - iDestruct "Hl" as (l' ?) "(-> & Hl' & Hl)".
+        wp_match; wp_load; wp_pures.
+        destruct (bool_decide (#x = #target)) eqn:?.
+        + wp_pures.
+          iApply "HPost".
+          cbn; rewrite (bool_decide_true_Zeqb _ _ Heqb0).
+          iExists l', hd'.
+          iFrame.
+          done.
+        + wp_pures.
+          destruct (bool_decide (Z.lt x target)) eqn:?; wp_pures.
+          * wp_bind (insert_list _); wp_load; wp_pures.
+            iApply ("IH" with "[Hl]"); [done|].
+            iNext.
+            iIntros (?) "Hr".
+            wp_store; wp_pure.
+            iApply "HPost".
+            unfold Insert_list.
+            rewrite (bool_decide_false_Zeqb _ _ Heqb0).
+            rewrite bool_decide_eq_true in Heqb1;
+              apply Z.ltb_lt in Heqb1;
+              rewrite Heqb1.
+            iExists l', r.
+            iFrame.
+            done.
+          * wp_alloc new as "Hnew"; wp_pure.
+            iApply "HPost".
+            unfold Insert_list;
+              specialize (bool_decide_false_Zeqb _ _ Heqb0) as ?;
+              rewrite bool_decide_eq_false in Heqb1;
+              assert (Z.le target x) by lia;
+              apply Z.leb_le in H0;
+              rewrite Z.leb_antisym in H0;
+              symmetry in H0;
+              apply negb_sym in H0;
+              cbn in H0;
+              rewrite H H0.
+            iExists new, (InjRV #l').
+            iFrame.
+            iSplitR; [done|].
+            iExists l', hd'.
+            iFrame.
+            done.
+    Qed.
+
+    Lemma insert_nary_tree_spec (t : nary_tree) (t_wf : nary_tree_wf_no_len b t) (v : val) (target : nat) :
+      {{{ is_node v t }}} insert_bplus_tree (v, #target)%V {{{ r, RET r; is_node r (Insert_nary_tree target t) }}}.
+    Proof using bpos.
+      iIntros (Φ) "Hv HPost".
+
+      iInduction t as [(low & high)|(low & high) ts] "IH" using nary_tree_ind' forall (v).
+      - iPoseProof (tree_leaf_token_leaf with "Hv") as (?) "->".
+        iDestruct "Hv" as (? ?) "(% & Hptr & Hlhd)".
+        assert (x = #ptr) by (unfold token_leaf_v in H; congruence); subst.
+        wp_rec; wp_load; wp_pures; wp_bind (insert_list _).
+        iApply (insert_list_spec with "Hlhd").
+        iNext.
+        iIntros (?) "Hr".
+        wp_load; wp_store.
+        iApply "HPost".
+        iExists ptr, r.
+        iFrame.
+        done.
+      - iPoseProof (tree_node_token_branch with "Hv") as (?) "->".
+        iDestruct "Hv" as (ptr lhd ns) "(% & Hptr & Hlhd & Hns)".
+        assert (x = #ptr) by (unfold token_branch_v in H; congruence); subst.
+        
+
     Admitted.
 
   End bplus_tree_proofs.
